Moved to a recent build of FStar and made progress on the elaboration system

src/Core.Environment.fst
@@ -1,8 +1,9 @@
 module Core.Environment
 
-open Util.Reader
-
+open Core.Name
 open Core.Ltt
+
+module M = FStar.OrdMap
 
 (**
 Represents a declaration.
@@ -20,34 +21,35 @@ just falling back on a list.
 NOTE: look at the [FStar.DM4F.StMap](https://github.com/FStarLang/FStar/blob/master/examples/dm4free/FStar.DM4F.StMap.fst)
 example--it uses `FStar.Map` in a STATE monad.
 *)
-type env = list (name * decl)
+abstract type env = name_map decl
 
 (** Look up a declaration within the typechecking
     environment. *)
-abstract val env_lookup : env -> name -> Tot (option decl)
-let rec env_lookup e n =
-  match e with
-  | [] -> None
-  | (sn,sd) :: xs -> if sn = n
-      then Some sd
-      else env_lookup xs n
+val env_lookup : env -> name -> Tot (option decl)
+let rec env_lookup e n = M.select n e
 
 (**
 `env_add` adds a declaration to an environment.
 *)
-abstract val env_add : env -> name -> decl -> Tot env
-let env_add e n d = (n,d) :: e
+val env_add : env -> name -> decl -> Tot env
+let env_add e n d = M.update n d e
 
 (**
 `env_init` initializes an environment using a
 list of tuples pairing a name and a declaration.
 *)
-abstract val env_init : list (name * decl) -> Tot env
-let env_init = id
+val env_init : list (name * decl) -> Tot env
+let env_init = List.Tot.fold_left
+  (fun envr (n,d) -> env_add envr n d) M.empty
 
 (**
 Predicate for checking if a name is in the environment.
 *)
 val env_has : env -> name -> Tot bool
-let rec env_has e n =
-  Option.isSome (env_lookup e n)
+let rec env_has e n = M.contains n e
+
+val env_has_in : env -> name -> decl -> Type0
+let env_has_in e n d =
+  match env_lookup e n with
+  | Some v -> v = d
+  | None -> false
