src/Core.Ltt.fst
@@ -4,90 +4,35 @@ open FStar.OrdSet
 open FStar.String
 open FStar.Tactics
 
-(**
-Represents an identifier.
+module N = Core.Name
 
-If there's a conflict during the capture-avoiding
-substitution process, the `index` value is
-incremented.
-*)
-type name = {
-  index : nat;
-  str : string;
-}
+(** `ltt` is the core logic that type-checking occurs within.
 
-(**
-Introduce a new name.
+    `binder` is a binder in the core logic.
 
-Initializes the name with `index` at `0`.
-*)
-val intro : string -> Tot name
-let intro s = {index=0;str=s}
+    NOTE: the docs for both of these types are together like
+    this because putting the binder docs where
+    [this wiki page](https://github.com/FStarLang/FStar/wiki/Generating-documentation-with-fsdoc-comments)
+    says to results in the F* subprocess for interactive
+    typechecking exiting.
 
-(**
-Increment the index of a name.
-*)
-val inc_name : name -> Tot name
-let inc_name n = { index = n.index+1; str = n.str }
-
-(**
-`type` is the core logic that type-checking occurs within.
-
-`binder` is a binder in the core logic.
-
-NOTE: the docs for both of these types are together like
-this because putting the binder docs where
-[this wiki page](https://github.com/FStarLang/FStar/wiki/Generating-documentation-with-fsdoc-comments)
-says to results in the F* subprocess for interactive
-typechecking exiting.
-
-TODO: ask about how to fix that.
-*)
+    TODO: ask about how to fix that. *)
 type ltt =
-  | Var : var:name -> ltt
+  | Var : var:N.name -> ltt
   | Universe : ltt
-  | Abs : bnd:binder -> var:name -> body:ltt -> ltt
+  | Abs : bnd:binder -> var:N.name -> body:ltt -> ltt
   | App : l:ltt -> r:ltt -> ltt
 and binder =
   | Pi : ltt -> binder
   | Lam : binder
 
-(**
-A total ordering on names.
-*)
-val name_order : name -> name -> Tot bool
-let name_order n1 n2 =
-  if n1.index = n1.index
-    then 0 <= compare n1.str n2.str
-    else n1.index > n2.index
-
-(*
-I can't figure out how to prove that string
-comparison is total, so I'm just making this
-an axiom.
-
-NOTE: if this is an `fsdoc` comment, it again
-seems to crash the F* subprocess for interactive
-typechecking.
-
-TODO: figure out how to fix that.
-*)
-assume NameOrderIsTotal: total_order name name_order
-
-(**
-A type alias for a set of names.
-
-Generally used when calculating free variables.
-*)
-type name_set = ordset name name_order
-
 (** Calculate the free variables in an `ltt` term. *)
-val free_variables : t:ltt -> Tot name_set
+val free_variables : t:ltt -> Tot N.name_set
 (** Calculate the free variables in a `ltt` binder. *)
-val binder_free_variables : binder -> Tot name_set
+val binder_free_variables : binder -> Tot N.name_set
 let rec free_variables t =
   match t with
-  | Var var -> singleton var
+  | Var v -> singleton v
   | Universe -> empty
   | Abs bnd var body ->
     let binder_fv = binder_free_variables bnd in
@@ -101,7 +46,7 @@ and binder_free_variables b =
 (**
 Predicate for checking if a name is free in a `ltt` term.
 *)
-val free_in : name -> ltt -> Tot bool
+val free_in : N.name -> ltt -> Tot bool
 let free_in v e = mem v (free_variables e)
 
 (**
@@ -122,11 +67,11 @@ removes `n` from `s` before recursing. This is done
 to show termination, but it's a quick hack that I
 should go back and fix if this project ever gets anywhere.
 *)
-val find_non_capturing_name : n:name -> s:name_set -> Tot name (decreases (size s))
+val find_non_capturing_name : n:N.name -> s:N.name_set -> Tot N.name (decreases (size s))
 let rec find_non_capturing_name n s =
   if mem n s
-    then let s': name_set = remove n s in
-         find_non_capturing_name (inc_name n) s'
+    then let s': N.name_set = remove n s in
+         find_non_capturing_name (N.inc_name n) s'
     else n
 
 (** Size metric for `ltt` terms. *)
@@ -151,7 +96,7 @@ Replaces all occurances of `replacee` with `substitute`.
 This is essentially a specialized version of `subst`;
 I created it bec
 *)
-private val replace_var : name -> name -> t:ltt -> Tot (ret:ltt{ltt_size ret = ltt_size t})
+private val replace_var : N.name -> N.name -> t:ltt -> Tot (ret:ltt{ltt_size ret = ltt_size t})
 let rec replace_var substitute replacee t =
   let rep = replace_var substitute replacee in
   match t with
@@ -171,13 +116,13 @@ let rec replace_var substitute replacee t =
 (**
 Perform capture-avoiding substitution of `arg` for `v` in  `bod`.
 *)
-val subst : arg:ltt -> v:name -> bod:ltt
+val subst : arg:ltt -> v:N.name -> bod:ltt
   -> Tot ltt (decreases %[ltt_size arg; ltt_size bod])
 
 (**
 Perform capture-avoiding substitution of `arg` for `v` in  `bnd`.
 *)
-val binder_subst : arg:ltt -> v:name -> bnd:binder
+val binder_subst : arg:ltt -> v:N.name -> bnd:binder
   -> Tot binder (decreases %[ltt_size arg; binder_size bnd])
 
 let rec subst arg v t =
@@ -222,9 +167,10 @@ and binder_alpha_eq b1 b2 =
   | _ -> false
 
 (** Assorted assertions. *)
+[@"opaque_to_smt"]
 let _ =
-  let x = intro "x" in
-  let y = intro "y" in
+  let x = N.intro "x" in
+  let y = N.intro "y" in
   let id = Abs Lam x (Var x) in
   let xy = Abs Lam x (Var y) in
   assert (subst (Universe) y xy = Abs Lam x (Universe));
