src/Core.Elab.fst
@@ -1,0 +1,245 @@
+module Core.Elab
+
+open Core.Name
+open Core.Ltt
+open Core.Environment
+module Tc = Core.Tc
+
+module UList = Util.UList
+open Util.Result
+
+open FStar.OrdMap
+
+(** The development calculus used during the elaboration process.
+
+    Adds `Guess` and `Hole` binders to the LTT calculus. *)
+type dev_ltt =
+  | DVar : var:name -> dev_ltt
+  | DUniverse : dev_ltt
+  | DAbs : bnd:dev_binder -> var:name -> body:dev_ltt -> dev_ltt
+  | DApp : l:dev_ltt -> r:dev_ltt -> dev_ltt
+and dev_binder =
+  | DPi : ty:dev_ltt -> dev_binder
+  | DLam : dev_binder
+  | Guess : dev_ltt -> dev_binder
+  | Hole : dev_binder
+
+(** Does the dev_ltt term contain anything that explicitly makes
+    it dev, and therefore not convertible to ltt. *)
+val is_ltt_dev : dev_ltt -> Tot bool
+
+(** Does the dev_binder term contain anything that explicitly makes
+    it dev, and therefore not convertible to binder. *)
+val is_binder_dev : dev_binder -> Tot bool
+
+let rec is_ltt_dev = function
+  | DVar _ -> false
+  | DUniverse -> false
+  | DAbs bnd var body -> is_binder_dev bnd || is_ltt_dev body
+  | DApp l r -> is_ltt_dev l || is_ltt_dev r
+and is_binder_dev = function
+  | DPi t -> is_ltt_dev t
+  | DLam -> false
+  | Guess _ -> true
+  | Hole -> true
+
+(** Convert a dev_ltt term that has no dev_ltt only members to ltt. *)
+val to_std_ltt : t:dev_ltt{not (is_ltt_dev t)} -> ltt
+(** Convert a dev_binder term that has no dev_binder only
+    members to binder. *)
+val to_std_binder : bnd:dev_binder{not (is_binder_dev bnd)} -> binder
+
+let rec to_std_ltt = function
+  | DVar v -> Var v
+  | DUniverse -> Universe
+  | DAbs bnd var body ->
+    Abs (to_std_binder bnd) var (to_std_ltt body)
+  | DApp l r ->
+    App (to_std_ltt l) (to_std_ltt r)
+and to_std_binder = function
+  | DPi t -> Pi (to_std_ltt t)
+  | DLam -> Lam
+
+(** An error that can occur during elaboration. *)
+type elab_err =
+  | TcErr of Tc.tc_err
+
+(** A mapping of names to `dev_ltt` terms. *)
+abstract type dev_ltt_context = name_map dev_ltt
+
+(** A unification problem. *)
+unopteq type unification_problem = {
+  context : dev_ltt_context;
+  e1 : ltt;
+  e2 : ltt
+}
+
+abstract type global_context = name_map decl
+
+type pattern_binding = unit
+
+(** The state of the elaboration monad. *)
+unopteq type elab_state = {
+  global_context : global_context;
+  local_context : list pattern_binding;
+  proof_term : dev_ltt;
+  unification_problems : list unification_problem;
+  hole_queue : UList.t name
+}
+
+(** A result from the elaboration monad. *)
+type elab_result a = Util.Result.result elab_err (elab_state * a)
+
+(** The representation of the elaboration monad. *)
+private let elab (a:Type) = elab_state -> M (elab_result a)
+
+(** Return implementation for ELAB. *)
+private val return_elab : a:Type -> a -> Tot (elab a)
+let return_elab a x = fun s -> Ok (s, x)
+
+(** Bind implementation for ELAB. *)
+private val bind_elab : a:Type -> b:Type
+                      -> x:elab a -> f:(a -> elab b) -> Tot (elab b)
+let bind_elab a b x f =
+  fun state ->
+    let res = x state in
+    bind_result res (fun (state', v) -> f v state')
+
+(** Retrieve the state of the ELAB monad. *)
+private val elab_get : unit -> Tot (elab elab_state)
+let elab_get (): Tot (elab elab_state) = fun state -> Ok (state, state)
+
+(** Put a new state into the ELAB monad. *)
+private val elab_put : elab_state -> Tot (elab unit)
+let elab_put s: elab unit = fun _ -> Ok (s, ())
+
+(** Raise an error in the ELAB monad. *)
+private val elab_raise : a:Type -> elab_err -> Tot (elab a)
+let elab_raise a err: elab a = fun _ -> Err err
+
+total reifiable reflectable new_effect {
+  ELAB : a:Type -> Effect
+  with repr = elab
+     ; bind = bind_elab
+     ; return = return_elab
+     ; get = elab_get
+     ; put = elab_put
+     ; raise = elab_raise
+}
+
+private type elab_post (a:Type) = elab_state -> elab_result a -> GTot Type0
+
+effect Elab (a:Type) (pre:ELAB?.pre) (post:elab_post a) =
+  ELAB a
+    (fun (state:elab_state) (p:ELAB?.post a) ->
+      pre state /\
+        (forall (r:elab_result a). pre state /\ post state r ==> p r))
+
+effect TrivElab (a:Type) =
+  Elab a (requires fun _ -> True) (ensures fun _ _ -> True)
+
+let get () = ELAB?.get ()
+let put (s:elab_state) = ELAB?.put s
+let raise (#a:Type) (err:elab_err) = ELAB?.raise a err
+
+reifiable reflectable new_effect {
+  DIV_ELAB : a:Type -> Effect
+  with repr = elab
+     ; bind = bind_elab
+     ; return = return_elab
+     ; get = elab_get
+     ; put = elab_put
+     ; raise = elab_raise
+}
+
+effect DivElab (a:Type) (pre:ELAB?.pre) (post:elab_post a) =
+  DIV_ELAB a
+    (fun (state:elab_state) (p:ELAB?.post a) ->
+      pre state /\
+        (forall (r:elab_result a). pre state /\ post state r ==> p r))
+
+sub_effect ELAB ~> DIV_ELAB {
+  lift = fun (a:Type) (rep:elab a) -> rep
+}
+
+val modify : f:(elab_state -> Tot elab_state) -> TrivElab unit
+let modify f =
+  let cur_state = get () in
+  let post_state = f cur_state in
+  put post_state
+
+(** Attempt a failable operation. *)
+val attempt : #a:Type -> #pre:ELAB?.pre -> #post:elab_post a -> (unit -> Elab a pre post) -> Elab (result elab_err a)
+  (requires pre)
+  (ensures fun state r ->
+    (match r with
+    | Err _ -> False
+    | Ok (state', inner_r) ->
+      (match inner_r with
+      | Err err -> state == state' /\ post state (Err err)
+      | Ok v -> post state (Ok (state', v)))))
+let attempt #a #pre #post eff =
+  let cur_state = get () in
+  let res = reify (eff ()) cur_state in
+  match res with
+  | Ok (state', v) -> put state'; Ok v
+  | Err err -> Err err
+
+(** Initialize a new proof state. *)
+val new_proof : global_context -> TrivElab unit
+let new_rpoof ctxt =
+  let n = mintro "initial" in
+  put ({
+    global_context = ctxt;
+    local_context = [];
+    proof_term = DAbs Hole n (DVar n);
+    unification_problems = [];
+    hole_queue = [n]
+  })
+
+val new_term : unit -> TrivElab unit
+let new_term () =
+  let n = mintro "initial" in
+  modify (fun cur_state -> { cur_state with
+    proof_term = DAbs Hole n (DVar n);
+    unification_problems = [];
+    hole_queue = [n]
+  })
+
+val focus : n:name -> Elab unit
+  (requires fun state -> List.mem n state.hole_queue)
+  (ensures fun _ r -> Ok? r)
+let focus n =
+  let state = get () in
+  let queue': UList.t name = n :: (UList.remove n state.hole_queue) in
+  put ({ state with hole_queue = queue' })
+
+val unfocus : unit -> Elab unit
+  (requires fun state -> not (List.isEmpty state.hole_queue))
+  (ensures fun _ r -> Ok? r)
+let unfocus () =
+  let state = get () in
+  let (n :: ns) = state.hole_queue in
+  let queue': UList.t name = UList.snoc ns n in
+  put ({ state with hole_queue = queue' })
+
+val new_hole : n:name -> Elab unit
+  (requires fun state -> not (List.mem n state.hole_queue))
+  (ensures fun _ r -> Ok? r)
+let new_hole n =
+  let state = get () in
+  put ({ state with hole_queue = n :: state.hole_queue })
+
+val next_hole : unit -> Elab name
+  (requires fun state -> not (List.isEmpty state.hole_queue))
+  (ensures fun state r -> Ok? r /\ fst (Ok?.value r) == state)
+let next_hole () = List.Tot.hd (get ()).hole_queue
+
+val remove_hole : unit -> Elab unit
+  (requires fun state -> not (List.isEmpty state.hole_queue))
+  (ensures fun _ r -> Ok? r)
+let remove_hole () =
+  let state = get () in
+  put ({ state with hole_queue = List.Tot.tl state.hole_queue })
+
+
