src/Core.Name.fst
@@ -1,0 +1,103 @@
+module Core.Name
+
+open FStar.OrdSet
+
+module M = FStar.OrdMap
+module O = FStar.Order
+
+(** Represents an identifier.
+
+    If there's a conflict during the capture-avoiding
+    substitution process, the `index` value is
+    incremented. *)
+type base_name = {
+  index : nat;
+  str : string;
+}
+
+(** Useful information about a name, such as
+    its origin. *)
+type name_sort =
+  | UserGen
+  | MachineGen
+
+(** A name used to identify something. *)
+type name = {
+  base : base_name;
+  sort : name_sort
+}
+
+(** Apply a modification to the base name. *)
+val mod_base_name : (base_name -> Tot base_name) -> name -> Tot name
+let mod_base_name f n = { sort = n.sort; base = f n.base }
+
+(** Introduce a new user-generated name.
+
+    Initializes the name with `index` at `0`. *)
+val intro : string -> Tot name
+let intro s = {
+  sort = UserGen;
+  base = {
+    str = s;
+    index = 0
+  }
+}
+
+(** Introduce a new machine-generated name. *)
+val mintro : string -> Tot name
+let mintro s = {
+  sort = MachineGen;
+  base = {
+    str = s;
+    index = 0
+  }
+}
+
+(** Increment the index of a name. *)
+val inc_name : name -> Tot name
+let inc_name = mod_base_name
+  (fun n -> { index = n.index+1; str = n.str })
+
+(** A total ordering on names. *)
+abstract val name_order : name -> name -> Tot bool
+let name_order n1 n2 =
+  let compare_sort s1 s2 =
+    let rank (s:name_sort): nat =
+      match s with
+      | UserGen -> 1
+      | MachineGen -> 0 in
+
+    O.compare_int (rank s1) (rank s2) in
+
+  let compare_string s1 s2 =
+    Order.order_from_int (String.compare s1 s2) in
+
+  let compare_name n1 n2 =
+    O.lex (compare_sort n1.sort n2.sort)
+      (fun () -> O.lex (O.compare_int n1.base.index n2.base.index)
+        (fun () -> compare_string n1.base.str n2.base.str)) in
+
+  O.gt (compare_name n1 n2)
+
+(*
+I can't figure out how to prove that string
+comparison is total, so I'm just making this
+an axiom.
+
+NOTE: if this is an `fsdoc` comment, it again
+seems to crash the F* subprocess for interactive
+typechecking.
+
+TODO: figure out how to fix that.
+*)
+assume NameOrderIsTotal: total_order name name_order
+
+let name_order_cmp: cmp name = name_order
+
+(** A type alias for a set of names.
+
+    Generally used when calculating free variables. *)
+let name_set: Type0 = ordset name name_order
+
+(** A type alias for a map from names to `a`. *)
+type name_map (a:Type) = M.ordmap name a name_order
