src/Util.Result.fst
@@ -1,0 +1,11 @@
+module Util.Result
+
+type result (b:Type) (a:Type) =
+  | Err : err:b -> result b a
+  | Ok : value:a -> result b a
+
+val bind_result : result 's 'a -> f:('a -> result 's 'b) -> result 's 'b
+let bind_result r f =
+  match r with
+  | Ok v -> f v
+  | Err err -> Err err
