fstar-env.nix
@@ -1,0 +1,37 @@
+{ pkgs ? (import <nixpkgs> {}) }:
+
+let inherit (pkgs) stdenv fetchFromGitHub z3 ocamlPackages makeWrapper; in
+
+pkgs.mkShell {
+  nativeBuildInputs = [ makeWrapper ];
+
+  buildInputs = with ocamlPackages; [
+    z3 ocaml findlib batteries menhir stdint
+    zarith camlp4 yojson pprint
+    ulex ocaml-migrate-parsetree process ppx_deriving ppx_deriving_yojson ocamlbuild
+  ];
+
+  /*makeFlags = [ "PREFIX=$(out)" ];
+
+  preBuild = ''
+    patchShebangs src/tools
+    patchShebangs bin
+  '';
+  buildFlags = "-C src/ocaml-output";
+
+  preInstall = ''
+    mkdir -p $out/lib/ocaml/${ocamlPackages.ocaml.version}/site-lib/fstarlib
+  '';
+  installFlags = "-C src/ocaml-output";
+  postInstall = ''
+    wrapProgram $out/bin/fstar.exe --prefix PATH ":" "${z3}/bin"
+  '';
+
+  meta = with stdenv.lib; {
+    description = "ML-like functional programming language aimed at program verification";
+    homepage = https://www.fstar-lang.org;
+    license = licenses.asl20;
+    platforms = with platforms; darwin ++ linux;
+    maintainers = with maintainers; [ gebner ];
+  };*/
+}
