fstar.nix
@@ -1,0 +1,64 @@
+{ stdenv, fetchFromGitHub, z3, ocamlPackages, makeWrapper, which, file }:
+
+stdenv.mkDerivation rec {
+  name = "fstar-${version}";
+  version = "commit-1aeb400"; 
+  src = fetchFromGitHub {
+    owner = "FStarLang";
+    repo = "FStar";
+    rev = "d510234e841715b5ba4debd2aa7214954e084a07";
+    sha256 = "12iwih61pksjskn5kdb6srb9v3v38wq7kz6dw5xnbgwb2vyi66fm";
+  };
+
+  nativeBuildInputs = [ makeWrapper ];
+
+  buildInputs = with ocamlPackages; [
+    file which
+    z3 ocaml findlib batteries menhir stdint
+    zarith camlp4 yojson pprint
+    ulex ocaml-migrate-parsetree process ppx_deriving ppx_deriving_yojson ocamlbuild
+  ];
+
+  makeFlags = [ "PREFIX=$(out)" ];
+
+  preBuild = ''
+    echo "OUT IS"
+    echo $out
+    patchShebangs src/tools
+    patchShebangs bin
+  '';
+  buildFlags = "-C src -j6 ocaml-fstar-ocaml";
+
+  /*installPhase = ''
+    mkdir -p $out/lib/ocaml/${ocamlPackages.ocaml.version}/site-lib/fstarlib
+    make -C src/ocaml-output -j6
+    make -C src -j6
+    wrapProgram $out/bin/fstar.exe --prefix PATH ":" "${z3}/bin"
+  '';*/
+  installPhase = ''
+    make -C ulib install-fstarlib install-fstar-tactics
+    mkdir -p $out/lib/ocaml/${ocamlPackages.ocaml.version}/site-lib/fstarlib
+    # mkdir -p $out/bin/
+    # cp bin/fstar.exe $out/bin/fstar.exe
+    ls bin/
+    make -C src/ocaml-output install PREFIX=$out
+    ls bin/
+    ls $out/bin/
+    wrapProgram $out/bin/fstar.exe --prefix PATH ":" "${z3}/bin"
+  '';
+  /*preInstall = ''
+    mkdir -p $out/lib/ocaml/${ocamlPackages.ocaml.version}/site-lib/fstarlib
+  '';
+  #installFlags = "-C src -j6 ocaml-fstar-ocaml";
+  postInstall = ''
+    wrapProgram $out/bin/fstar.exe --prefix PATH ":" "${z3}/bin"
+  '';*/
+
+  meta = with stdenv.lib; {
+    description = "ML-like functional programming language aimed at program verification";
+    homepage = https://www.fstar-lang.org;
+    license = licenses.asl20;
+    platforms = with platforms; darwin ++ linux;
+    maintainers = with maintainers; [ gebner ];
+  };
+}
