pinned-nixpkgs.nix
@@ -2,6 +2,7 @@ let
    hostPkgs = import <nixpkgs> {};
    # Generated through:
    # nix-shell -p nix-prefetch-git --run "nix-prefetch-git  https://github.com/nixos/nixpkgs-channels.git --rev {rev} > nixpkgs-version.json"
+   # where {rev} is the desired revision.
    pinnedVersion = hostPkgs.lib.importJSON ./nixpkgs-version.json;
 
    pinnedPkgs = hostPkgs.fetchFromGitHub {
