shell.nix
@@ -2,10 +2,12 @@ let pinned-nixpkgs-path = import ./pinned-nixpkgs.nix;
     pinned-pkgs = import pinned-nixpkgs-path {};
 in { pkgs ? pinned-pkgs }: # if I ever need to override stuff
 
-with pkgs;
-
-mkShell {
+let
+  z3 = pkgs.z3;
+  fstar = pkgs.callPackage ./fstar.nix {};
+in pkgs.mkShell {
   buildInputs = [
-    fstar z3
+    fstar
+    z3
   ];
 }
